cfrontend/Csem.v
@@ -115,7 +115,7 @@ Inductive alloc_variables: env -> mem ->
       alloc_variables e m nil e m
   | alloc_variables_cons:
       forall e m id ty vars m1 b1 m2 e2,
-      Mem.alloc m 0 (sizeof ge ty) = (m1, b1) ->
+      Mem.alloc m 0 (sizeof ge ty) = Some (m1, b1) ->
       alloc_variables (PTree.set id (b1, ty) e) m1 vars e2 m2 ->
       alloc_variables e m ((id, ty) :: vars) e2 m2.
 
@@ -789,6 +789,7 @@ Inductive sstep: state -> trace -> state -> Prop :=
       list_norepet (var_names (fn_params f) ++ var_names (fn_vars f)) ->
       alloc_variables empty_env m (f.(fn_params) ++ f.(fn_vars)) e m1 ->
       bind_parameters e m1 f.(fn_params) vargs m2 ->
+      Mem.alloc_flag m = true ->
       sstep (Callstate vf vargs k m)
          E0 (State f f.(fn_body) k e m2)
 
