backend/Deadcodeproof.v
@@ -52,7 +52,9 @@ Record magree (m1 m2: mem) (P: locset) : Prop := mk_magree {
     memval_lessdef (ZMap.get ofs (PMap.get b (Mem.mem_contents m1)))
                    (ZMap.get ofs (PMap.get b (Mem.mem_contents m2)));
   ma_nextblock:
-    Mem.nextblock m2 = Mem.nextblock m1
+    Mem.nextblock m2 = Mem.nextblock m1;
+  ma_alloc_flag:
+    Mem.alloc_flag m2 = Mem.alloc_flag m1
 }.
 
 Lemma magree_monotone:
@@ -73,6 +75,7 @@ Proof.
 - exploit mi_memval; eauto. unfold inject_id; eauto.
   rewrite Z.add_0_r. auto.
 - auto.
+- congruence.
 Qed.
 
 Lemma magree_extends:
@@ -174,6 +177,9 @@ Proof.
 - rewrite (Mem.nextblock_storebytes _ _ _ _ _ H0).
   rewrite (Mem.nextblock_storebytes _ _ _ _ _ ST2).
   eapply ma_nextblock; eauto.
+- apply Mem.storebytes_alloc_flag in H0.
+  apply Mem.storebytes_alloc_flag in ST2.
+  destruct H. congruence.
 Qed.
 
 Lemma magree_store_parallel:
@@ -217,6 +223,7 @@ Proof.
 + eapply ma_memval; eauto. eapply Mem.perm_storebytes_2; eauto.
 - rewrite (Mem.nextblock_storebytes _ _ _ _ _ H0).
   eapply ma_nextblock; eauto.
+- apply Mem.storebytes_alloc_flag in H0. destruct H. congruence.
 Qed.
 
 Lemma magree_store_left:
@@ -265,6 +272,8 @@ Proof.
   rewrite (Mem.free_result _ _ _ _ _ H0).
   rewrite (Mem.free_result _ _ _ _ _ FREE).
   simpl. eapply ma_nextblock; eauto.
+- apply Mem.free_alloc_flag in H0.
+  apply Mem.free_alloc_flag in FREE. destruct H. congruence.
 Qed.
 
 Lemma magree_valid_access:
@@ -1127,9 +1136,10 @@ Proof.
   intros MATCH. eapply source_invariant_fsim; eauto using rtl_vamatch. revert MATCH.
   fsim eapply forward_simulation_step with (match_states := match_states prog se1);
     cbn in *; subst.
-- destruct 1. cbn. CKLR.uncklr. destruct H as [vf|]; try congruence.
-  eapply (Genv.is_internal_transf_partial_id MATCH).
-  intros [|] [|] TFD; monadInv TFD; auto.
+(* - destruct 1. cbn. CKLR.uncklr. destruct H as [vf|]; try congruence. *)
+(*   eapply (Genv.is_internal_transf_partial_id MATCH). *)
+(*   intros [|] [|] TFD; monadInv TFD; auto. *)
+- destruct f1; monadInv H; reflexivity.
 - intros q1 q2 s1 Hq (Hs1 & _).
   eapply transf_initial_states; eauto.
 - intros s1 s2 r1 Hs (Hr1 & _).
