cklr/Join.v
@@ -1,0 +1,664 @@
+From compcert Require Import
+     AST Coqlib Maps Values Integers Errors Events
+     LanguageInterface Smallstep Globalenvs Memory Floats.
+Require Import Ctypes Cop Clight.
+
+Local Notation "a # b" := (PMap.get b a) (at level 1).
+
+Require Import LogicalRelations.
+Require Import OptionRel.
+Require Import Lia.
+
+Section JOIN.
+
+  Inductive contents_join: block -> Z -> mem -> mem -> mem -> Prop  :=
+  | contents_join_l:
+    forall m1 m2 m b ofs,
+      ~Mem.perm m1 b ofs Max Nonempty ->
+      (forall k p, Mem.perm m2 b ofs k p <-> Mem.perm m b ofs k p) ->
+      ZMap.get ofs m1.(Mem.mem_contents)#b = Undef ->
+      ZMap.get ofs m2.(Mem.mem_contents)#b =ZMap.get ofs m.(Mem.mem_contents)#b ->
+      Mem.valid_block m2 b ->
+      contents_join b ofs m1 m2 m
+  | contents_join_r:
+    forall m1 m2 m b ofs,
+      ~Mem.perm m2 b ofs Max Nonempty ->
+      (forall k p, Mem.perm m1 b ofs k p <-> Mem.perm m b ofs k p) ->
+      ZMap.get ofs m2.(Mem.mem_contents)#b = Undef ->
+      ZMap.get ofs m1.(Mem.mem_contents)#b =ZMap.get ofs m.(Mem.mem_contents)#b ->
+      Mem.valid_block m1 b ->
+      contents_join b ofs m1 m2 m.
+
+  Inductive alloc_flag_join: mem -> mem -> mem -> Prop :=
+  | alloc_flag_join_l:
+    forall m m1 m2,
+      Mem.alloc_flag m = false ->
+      Mem.alloc_flag m1 = true ->
+      Mem.alloc_flag m2 = true ->
+      (Mem.nextblock m <= Mem.nextblock m1)%positive ->
+      alloc_flag_join m m1 m2
+  | alloc_flag_join_r:
+    forall m m1 m2,
+      Mem.alloc_flag m1 = true ->
+      Mem.alloc_flag m = false ->
+      Mem.alloc_flag m2 = true ->
+      (Mem.nextblock m <= Mem.nextblock m1)%positive ->
+      alloc_flag_join m1 m m2
+  | alloc_flag_join_x:
+    forall m1 m2 m,
+      Mem.alloc_flag m1 = false ->
+      Mem.alloc_flag m2 = false ->
+      Mem.alloc_flag m = false ->
+      alloc_flag_join m1 m2 m.
+
+  Record join (m1 m2 m: mem) : Prop :=
+    mk_join {
+        mjoin_contents: forall b ofs, contents_join b ofs m1 m2 m;
+        mjoin_nextblock: Mem.nextblock m = Pos.max (Mem.nextblock m1) (Mem.nextblock m2);
+        mjoin_alloc_flag: alloc_flag_join m1 m2 m;
+      }.
+
+End JOIN.
+
+Hint Constructors  alloc_flag_join contents_join.
+
+Section JOIN_PROP.
+
+  Lemma join_commutative m1 m2 m:
+    join m1 m2 m -> join m2 m1 m.
+  Proof.
+    intros H. inv H. constructor.
+    - intros. specialize (mjoin_contents0 b ofs).
+      inv mjoin_contents0; eauto.
+    - now rewrite Pos.max_comm.
+    - inv mjoin_alloc_flag0; eauto.
+  Qed.
+
+  Lemma join_associative m1 m2 m3 m12 m23 m123:
+    join m1 m2 m12 -> join m12 m3 m123 -> join m2 m3 m23 -> join m1 m23 m123.
+  Proof.
+    intros A B C. inv A. inv B. inv C. constructor.
+    - intros b ofs.
+      specialize (mjoin_contents0 b ofs).
+      specialize (mjoin_contents1 b ofs).
+      specialize (mjoin_contents2 b ofs).
+      inv mjoin_contents0; inv mjoin_contents1; inv mjoin_contents2.
+      + apply contents_join_l; eauto; try congruence.
+        intros. rewrite <- H10. eauto.
+        unfold Mem.valid_block, Plt in *.
+        rewrite mjoin_nextblock2. lia.
+      + apply contents_join_l; eauto; try congruence.
+        intros. rewrite <- H5. rewrite <- H10. rewrite <- H0 in H4. split.
+  Admitted.
+
+End JOIN_PROP.
+
+Section JOIN_PROP.
+
+  Variable (m: mem).
+
+  Instance valid_pointer_join:
+    Monotonic
+      (@Mem.valid_pointer)
+      (join m ++> - ==> - ==> leb).
+  Proof.
+    do 4 rstep. destruct Mem.valid_pointer eqn: X; try easy.
+    cbn. rewrite !Mem.valid_pointer_nonempty_perm in *.
+    rename x0 into b. rename x1 into ofs.
+    destruct H. specialize (mjoin_contents0 b ofs). inv mjoin_contents0.
+    - apply H0. apply X.
+    - exfalso. apply H. eauto with mem.
+  Qed.
+
+  Instance weak_valid_pointer_join:
+    Monotonic
+      (@Mem.weak_valid_pointer)
+      (join m ++> - ==> - ==> leb).
+  Proof.
+    unfold Mem.weak_valid_pointer. do 4 rstep.
+    destruct orb eqn: X.
+    - simpl. rewrite orb_true_iff in *.
+      destruct X; [ left | right ]; apply valid_pointer_join in H.
+      specialize (H x0 x1). rewrite H0 in H. eauto.
+      specialize (H x0 (x1 - 1)%Z). rewrite H0 in H. eauto.
+    - easy.
+  Qed.
+
+  Instance bool_val_join:
+    Monotonic
+      (@bool_val)
+      (- ==> - ==> join m ++> option_le eq).
+  Proof. unfold bool_val. rauto. Qed.
+
+  Instance sem_unary_operation_join:
+    Monotonic
+      (@sem_unary_operation)
+      (- ==> - ==> - ==> join m ++> option_le eq).
+  Proof.
+    unfold sem_unary_operation.
+    unfold sem_notbool, sem_notint, sem_neg, sem_absfloat.
+    repeat rstep. f_equal. congruence.
+  Qed.
+
+  Instance sem_cast_join:
+    Monotonic
+      (@Cop.sem_cast)
+      (- ==> - ==> - ==> join m ++> option_le eq).
+  Proof. unfold Cop.sem_cast. rauto. Qed.
+
+  Instance sem_binarith_join:
+    Monotonic
+      (@Cop.sem_binarith)
+      (- ==> - ==> - ==> - ==> - ==> - ==> - ==> - ==> join m ++> option_le eq).
+  Proof. unfold Cop.sem_binarith. rauto. Qed.
+
+  Instance cmp_ptr_join:
+    Related
+      (@Cop.cmp_ptr)
+      (@Cop.cmp_ptr)
+      (join m ++> - ==> - ==> - ==> option_le eq).
+  Proof.
+    rstep. rstep. rstep. rstep. rstep.
+    unfold Cop.cmp_ptr. rstep. rstep. rewrite H0. reflexivity. rstep.
+    - rstep. unfold Val.cmplu_bool. repeat rstep.
+      destruct eq_block; repeat rstep.
+    - rstep. unfold Val.cmpu_bool. repeat rstep.
+      destruct eq_block; repeat rstep.
+  Qed.
+
+  Instance sem_cmp_join:
+    Monotonic
+      (@Cop.sem_cmp)
+      (- ==> - ==> - ==> - ==> - ==> join m ++> option_le eq).
+  Proof. unfold Cop.sem_cmp. repeat rstep. Qed.
+
+  Instance sem_binary_operation_join:
+    Monotonic
+      (@sem_binary_operation)
+      (- ==> - ==> - ==> - ==> - ==> - ==> join m ++> option_le eq).
+  Proof.
+    unfold sem_binary_operation.
+    unfold
+      Cop.sem_add,
+      Cop.sem_add_ptr_int,
+      Cop.sem_add_ptr_long,
+      Cop.sem_sub,
+      Cop.sem_mul,
+      Cop.sem_div,
+      Cop.sem_mod,
+      Cop.sem_and,
+      Cop.sem_or,
+      Cop.sem_xor,
+      Cop.sem_shl,
+      Cop.sem_shr.
+    repeat rstep.
+  Qed.
+
+  Lemma perm_join m1 m2 b ofs k p:
+    join m m1 m2 ->
+    Mem.perm m1 b ofs k p ->
+    Mem.perm m2 b ofs k p.
+  Proof.
+    intros HM H. inv HM. specialize (mjoin_contents0 b ofs).
+    inv mjoin_contents0.
+    - apply H1. apply H.
+    - exfalso. apply H0. eauto with mem.
+  Qed.
+
+  Lemma range_perm_join m1 m2 b lo hi k p:
+    join m m1 m2 ->
+    Mem.range_perm m1 b lo hi k p ->
+    Mem.range_perm m2 b lo hi k p.
+  Proof.
+    intros HM H ofs X. specialize (H _ X).
+    eauto using perm_join.
+  Qed.
+
+  Instance load_join:
+    Monotonic
+      (@Mem.load)
+      (- ==> join m ++> - ==> - ==> option_le eq).
+  Proof.
+    repeat rstep. destruct Mem.load eqn: X; try constructor.
+    rename x1 into b. rename x2 into ofs. rename x into ch.
+    rename x0 into m1. rename y into m2.
+    exploit Mem.load_valid_access. eauto. intros [A B].
+    exploit Mem.valid_access_load. split. eapply range_perm_join; eauto. apply B.
+    intros [w Y]. rewrite Y. constructor.
+    exploit Mem.load_result. apply X.
+    exploit Mem.load_result. apply Y. intros -> ->.
+    f_equal. apply Mem.getN_exten.
+    intros i Hi. destruct H. specialize (mjoin_contents0 b i).
+    inv mjoin_contents0; eauto.
+    exfalso. apply H. exploit A. instantiate (1 := i).
+    rewrite <- size_chunk_conv in Hi. exact Hi.
+    eauto with mem.
+  Qed.
+
+  Instance loadv_join:
+    Monotonic
+      (@Mem.loadv)
+      (- ==> join m ++> - ==> option_le eq).
+  Proof. unfold Mem.loadv. repeat rstep. Qed.
+
+  Instance deref_loc_join a:
+    Monotonic
+      (@deref_loc a)
+      (join m ++> - ==> - ==> - ==> impl).
+  Proof.
+    repeat rstep. intros A. inv A; eauto using @deref_loc_reference, @deref_loc_copy.
+    transport H1. subst. eapply deref_loc_value; eauto.
+  Qed.
+
+  Lemma get_setN_inside:
+    forall vl p q c,
+      p <= q < p + Z.of_nat (length vl) ->
+      (ZMap.get q (Mem.setN vl p c)) = nth (Z.to_nat (q - p)) vl Undef.
+  Proof.
+    induction vl; intros.
+    simpl in H. lia.
+    simpl length in H. rewrite Nat2Z.inj_succ in H. simpl.
+    destruct (zeq p q).
+    - subst q. rewrite Mem.setN_outside by lia. rewrite ZMap.gss.
+      replace (p - p) with 0 by lia. reflexivity.
+    - rewrite IHvl by lia. destruct H as [A B].
+      replace (q - p) with (Z.succ (q - p - 1)) by lia.
+      rewrite Z2Nat.inj_succ. 2: lia.
+      f_equal. f_equal. lia.
+  Qed.
+
+  Instance store_join:
+    Monotonic
+      (@Mem.store)
+      (- ==> join m ++> - ==> - ==> - ==> option_le (join m)).
+  Proof.
+    repeat rstep. destruct Mem.store eqn: X; try constructor.
+    rename x into ch. rename x1 into b. rename x2 into ofs. rename x3 into v.
+    rename x0 into m1. rename y into m2.
+    exploit Mem.store_valid_access_3; eauto. intros [A B].
+    edestruct Mem.valid_access_store as [n Y]. split. 2: eauto.
+    eapply range_perm_join; eauto.
+    rewrite Y. constructor.
+    constructor.
+    - intros bx ox. destruct H.
+      specialize (mjoin_contents0 bx ox). inv mjoin_contents0.
+      + apply contents_join_l; eauto.
+        * intros k p. specialize (H0 k p).
+          assert (P1: Mem.perm m0 bx ox k p <-> Mem.perm m1 bx ox k p).
+          split; eauto with mem.
+          assert (P2: Mem.perm n bx ox k p <-> Mem.perm m2 bx ox k p).
+          split; eauto with mem.
+          rewrite P1. rewrite H0. symmetry. apply P2.
+        * exploit Mem.store_mem_contents. apply X. intros ->.
+          exploit Mem.store_mem_contents. apply Y. intros ->.
+          destruct (PMap.elt_eq b bx).
+          -- subst. rewrite !PMap.gss.
+             destruct (zlt ox ofs).
+             ++ now rewrite !Mem.setN_outside by lia.
+             ++ destruct (zle (ofs + Z.of_nat (length (encode_val ch v))) ox).
+                now rewrite !Mem.setN_outside by lia.
+                now rewrite !get_setN_inside by lia.
+          -- rewrite !PMap.gso; eauto.
+        * eauto with mem.
+      + apply contents_join_r; eauto.
+        * intros P. apply H. eauto with mem.
+        * intros k p.
+          assert (P: Mem.perm n bx ox k p <-> Mem.perm m2 bx ox k p).
+          split; eauto with mem.
+          rewrite P. eauto.
+        * exploit Mem.store_mem_contents. apply X. intros ->.
+          destruct (PMap.elt_eq b bx).
+          -- subst. rewrite PMap.gss.
+             destruct (zlt ox ofs).
+             ++ now rewrite !Mem.setN_outside by lia.
+             ++ destruct (zle (ofs + Z.of_nat (length (encode_val ch v))) ox).
+                now rewrite !Mem.setN_outside by lia.
+                specialize (A ox).
+                exploit A.
+                rewrite encode_val_length in g0.
+                rewrite <- size_chunk_conv in g0. lia.
+                intros. exfalso. eauto with mem.
+          -- rewrite PMap.gso; eauto.
+        * rewrite H2.
+          exploit Mem.store_mem_contents. apply Y. intros ->.
+          destruct (PMap.elt_eq b bx).
+          -- subst. rewrite PMap.gss.
+             destruct (zlt ox ofs).
+             ++ now rewrite !Mem.setN_outside by lia.
+             ++ destruct (zle (ofs + Z.of_nat (length (encode_val ch v))) ox).
+                now rewrite !Mem.setN_outside by lia.
+                specialize (A ox).
+                exploit A.
+                rewrite encode_val_length in g0.
+                rewrite <- size_chunk_conv in g0. lia.
+                intros. exfalso. eauto with mem.
+          -- rewrite PMap.gso; eauto.
+    - destruct H.
+      apply Mem.nextblock_store in X.
+      apply Mem.nextblock_store in Y. congruence.
+    - destruct H.
+      exploit Mem.nextblock_store. apply X. intros C.
+      apply Mem.store_alloc_flag in X.
+      apply Mem.store_alloc_flag in Y.
+      inv mjoin_alloc_flag0.
+      + apply alloc_flag_join_l; eauto. congruence.
+      + apply alloc_flag_join_r; eauto. congruence.
+      + apply alloc_flag_join_x; eauto.
+  Qed.
+
+  Instance storev_join:
+    Monotonic
+      (@Mem.storev)
+      (- ==> join m ++> - ==> - ==> option_le (join m)).
+  Proof. unfold Mem.storev. repeat rstep. Qed.
+
+  Transparent Mem.loadbytes Mem.storebytes.
+  Instance loadbytes_join:
+    Monotonic
+      (@Mem.loadbytes)
+      (join m ++> - ==> - ==> - ==> option_le eq).
+  Proof.
+    repeat rstep. destruct Mem.loadbytes eqn: X; try constructor.
+    unfold Mem.loadbytes in *.
+    rename x0 into b. rename x1 into ofs. rename x2 into sz.
+    rename x into m1. rename y into m2.
+    destruct (Mem.range_perm_dec m1 b ofs (ofs + sz) Cur Readable); inv X.
+    destruct Mem.range_perm_dec.
+    - constructor. apply Mem.getN_exten. intros i Hi.
+      destruct H. specialize (mjoin_contents0 b i).
+      inv mjoin_contents0; eauto.
+      specialize (r i). exploit r.
+      {
+        destruct (zle 0 sz).
+        + rewrite Z2Nat.id in Hi; eauto.
+        + rewrite Z_to_nat_neg in Hi; lia.
+      }
+      intros. exfalso. eauto with mem.
+    - exfalso. destruct H.  apply n. intros x Hx.
+      specialize (mjoin_contents0 b x). inv mjoin_contents0.
+      + apply H0. eauto.
+      + exfalso. apply H. eauto with mem.
+  Qed.
+
+  Instance storebytes_join:
+    Monotonic
+      (@Mem.storebytes)
+      (join m ++> - ==> - ==> - ==> option_le (join m)).
+  Proof.
+    repeat rstep. destruct Mem.storebytes eqn: X; try constructor.
+    rename x0 into b. rename x1 into ofs. rename x2 into vl.
+    rename x into m1. rename y into m2.
+    pose proof (Mem.storebytes_range_perm _ _ _ _ _ X) as A.
+    edestruct Mem.range_perm_storebytes as (n & Y).
+    eapply range_perm_join; eauto.  rewrite Y. constructor.
+    constructor.
+    - intros bx ox. destruct H.
+      specialize (mjoin_contents0 bx ox). inv mjoin_contents0.
+      + apply contents_join_l; eauto.
+        * intros k p. specialize (H0 k p).
+          assert (P1: Mem.perm m0 bx ox k p <-> Mem.perm m1 bx ox k p).
+          split; eauto with mem.
+          assert (P2: Mem.perm n bx ox k p <-> Mem.perm m2 bx ox k p).
+          split; eauto with mem.
+          rewrite P1. rewrite H0. symmetry. apply P2.
+        * exploit Mem.storebytes_mem_contents. apply X. intros ->.
+          exploit Mem.storebytes_mem_contents. apply Y. intros ->.
+          destruct (PMap.elt_eq b bx).
+          -- subst. rewrite !PMap.gss.
+             destruct (zlt ox ofs).
+             ++ now rewrite !Mem.setN_outside by lia.
+             ++ destruct (zle (ofs + Z.of_nat (Datatypes.length vl)) ox).
+                now rewrite !Mem.setN_outside by lia.
+                now rewrite !get_setN_inside by lia.
+          -- rewrite !PMap.gso; eauto.
+        * eauto with mem.
+      + apply contents_join_r; eauto.
+        * intros P. apply H. eauto with mem.
+        * intros k p.
+          assert (P: Mem.perm n bx ox k p <-> Mem.perm m2 bx ox k p).
+          split; eauto with mem.
+          rewrite P. eauto.
+        * exploit Mem.storebytes_mem_contents. apply X. intros ->.
+          destruct (PMap.elt_eq b bx).
+          -- subst. rewrite PMap.gss.
+             destruct (zlt ox ofs).
+             ++ now rewrite !Mem.setN_outside by lia.
+             ++ destruct (zle (ofs + Z.of_nat (Datatypes.length vl)) ox).
+                now rewrite !Mem.setN_outside by lia.
+                specialize (A ox). exploit A. lia.
+                intros. exfalso. eauto with mem.
+          -- rewrite PMap.gso; eauto.
+        * rewrite H2.
+          exploit Mem.storebytes_mem_contents. apply Y. intros ->.
+          destruct (PMap.elt_eq b bx).
+          -- subst. rewrite PMap.gss.
+             destruct (zlt ox ofs).
+             ++ now rewrite !Mem.setN_outside by lia.
+             ++ destruct (zle (ofs + Z.of_nat (Datatypes.length vl)) ox).
+                now rewrite !Mem.setN_outside by lia.
+                specialize (A ox). exploit A. lia.
+                intros. exfalso. eauto with mem.
+          -- rewrite PMap.gso; eauto.
+    - destruct H.
+      apply Mem.nextblock_storebytes in X.
+      apply Mem.nextblock_storebytes in Y. congruence.
+    - destruct H.
+      exploit Mem.nextblock_storebytes. apply X. intros C.
+      apply Mem.storebytes_alloc_flag in X.
+      apply Mem.storebytes_alloc_flag in Y.
+      inv mjoin_alloc_flag0.
+      + apply alloc_flag_join_l; eauto. congruence.
+      + apply alloc_flag_join_r; eauto. congruence.
+      + apply alloc_flag_join_x; eauto.
+  Qed.
+
+  Opaque Mem.loadbytes Mem.storebytes.
+
+  Instance assign_loc_join:
+    Monotonic
+      (@assign_loc)
+      (- ==> - ==> join m ++> - ==> - ==> - ==> set_le (join m)).
+  Proof.
+    repeat rstep. intros ma A. inv A.
+    - transport H1. eexists; split; eauto.
+      eapply assign_loc_value; eauto.
+    - transport H4. subst.
+      transport H5.
+      eexists; split; eauto.
+      eapply assign_loc_copy; eauto.
+  Qed.
+
+  Instance free_join:
+    Monotonic
+      (@Mem.free)
+      (join m ++> - ==> - ==> - ==> option_le (join m)).
+  Proof.
+    repeat rstep.
+    rename x0 into b. rename x1 into lo. rename x2 into hi.
+    rename x into m1. rename y into m2.
+    destruct (Mem.free m1 b lo hi) eqn: HF; try constructor.
+    edestruct Mem.range_perm_free.
+    eapply range_perm_join; eauto.
+    eapply Mem.free_range_perm; eauto.
+    rewrite e. constructor. constructor.
+    - intros bx ox. destruct H.
+      specialize (mjoin_contents0 bx ox). inv mjoin_contents0.
+      + apply contents_join_l; eauto.
+        * intros k p. specialize (H0 k p). split; intros.
+          -- exploit Mem.perm_free_3. apply HF. eauto. intros A.
+             eapply Mem.perm_free_1; eauto.
+             destruct (peq bx b). 2: eauto.
+             destruct (zle lo ox). 2: lia.
+             destruct (zlt ox hi). 2: lia.
+             subst. exfalso. eapply Mem.perm_free_2. apply HF.
+             instantiate (1 := ox). lia. eauto.
+             apply H0; eauto.
+          -- exploit Mem.perm_free_3. apply e. eauto. intros.
+             eapply Mem.perm_free_1; eauto.
+             destruct (peq bx b). 2: eauto.
+             destruct (zle lo ox). 2: lia.
+             destruct (zlt ox hi). 2: lia.
+             subst. exfalso. eapply Mem.perm_free_2. apply e.
+             instantiate (1 := ox). lia. eauto.
+             apply H0; eauto.
+        * eapply Mem.free_result in HF.
+          eapply Mem.free_result in e. subst.
+          apply H2.
+        * eauto with mem.
+      + apply contents_join_r; eauto.
+        * intros A. apply H.
+          eapply Mem.perm_free_3; eauto.
+        * intros k p. specialize (H0 k p). rewrite H0.
+          assert (bx <> b \/ ox < lo \/ hi <= ox).
+          {
+             destruct (peq bx b). 2: eauto.
+             destruct (zle lo ox). 2: lia.
+             destruct (zlt ox hi). 2: lia.
+             exfalso. subst. apply H.
+             apply Mem.free_range_perm in HF.
+             eauto with mem.
+          }
+          split; intros.
+          -- eapply Mem.perm_free_1; eauto.
+          -- eapply Mem.perm_free_3; eauto.
+        * eapply Mem.free_result in HF. subst. apply H1.
+        * eapply Mem.free_result in HF.
+          eapply Mem.free_result in e. subst.
+          apply H2.
+    - destruct H.
+      apply Mem.nextblock_free in HF.
+      apply Mem.nextblock_free in e. congruence.
+    - destruct H.
+      exploit Mem.nextblock_free. apply HF. intros C.
+      apply Mem.free_alloc_flag in HF.
+      apply Mem.free_alloc_flag in e.
+      inv mjoin_alloc_flag0.
+      + apply alloc_flag_join_l; eauto. congruence.
+      + apply alloc_flag_join_r; eauto. congruence.
+      + apply alloc_flag_join_x; eauto.
+  Qed.
+
+  Instance free_list_join:
+    Monotonic
+      (@Mem.free_list)
+      (join m ++> - ==> option_le (join m)).
+  Proof.
+    repeat rstep. revert x y H. rename x0 into l. induction l.
+    - constructor. eauto.
+    - intros. destruct a. destruct p.
+      cbn. destruct (Mem.free x b z0 z) eqn: HX. 2: constructor.
+      transport HX. rewrite H0. eauto.
+  Qed.
+
+  Local Transparent Mem.alloc.
+  Instance alloc_join:
+    Monotonic
+      (@Mem.alloc)
+      (join m ++> - ==> - ==> option_le ((join m) * eq)).
+  Proof.
+    repeat rstep.
+    rename x0 into lo. rename x1 into hi.
+    rename x into m1. rename y into m2.
+    destruct (Mem.alloc m1 lo hi) eqn: HA; try constructor.
+    destruct p as (m1' & b1).
+    destruct H.
+    exploit Mem.alloc_flag_alloc1; eauto. intros A.
+    inv mjoin_alloc_flag0; try congruence.
+    edestruct Mem.alloc_succeed as [[m2' b2] HB].
+    apply H1. rewrite HB. constructor.
+    assert (HNB: Mem.nextblock m1 = Mem.nextblock m2).
+    { apply Pos.max_r in H2. congruence. }
+    assert (X: b1 = b2).
+    {
+      apply Mem.alloc_result in HA.
+      apply Mem.alloc_result in HB.
+      congruence.
+    }
+    subst; split; cbn; eauto.
+    - constructor.
+      + intros bx ox. specialize (mjoin_contents0 bx ox).
+        inv mjoin_contents0.
+        * apply contents_join_l; eauto.
+          -- intros k p.
+             destruct (peq bx b2).
+             ++ subst. split; intros.
+                ** exploit Mem.perm_alloc_inv. apply HA. eauto.
+                   destruct eq_block; try easy.
+                   intros. eauto with mem.
+                ** exploit Mem.perm_alloc_inv. apply HB. eauto.
+                   destruct eq_block; try easy.
+                   intros. eauto with mem.
+             ++ split; intros.
+                ** exploit Mem.perm_alloc_4. apply HA. all: eauto.
+                   intros. eapply Mem.perm_alloc_1; eauto.
+                   apply H4. eauto.
+                ** exploit Mem.perm_alloc_4. apply HB. all: eauto.
+                   intros. eapply Mem.perm_alloc_1; eauto.
+                   apply H4. eauto.
+          -- unfold Mem.alloc in HA, HB.
+             rewrite A in HA. inv HA.
+             rewrite H1 in HB. inv HB. cbn.
+             rewrite HNB.
+             destruct (peq bx (Mem.nextblock m2)).
+             ++ subst. rewrite !PMap.gss. reflexivity.
+             ++ rewrite !PMap.gso; eauto.
+          -- eauto with mem.
+        * assert (bx <> b2).
+          {
+            intros X. subst. unfold Mem.valid_block, Plt in H7.
+            apply Mem.alloc_result in HB. subst.
+            rewrite HNB in *. lia.
+          }
+          apply contents_join_r; eauto.
+          -- intros X. apply H3. eauto with mem.
+          -- intros k p. rewrite H4.
+             split; intros; eauto with mem.
+          -- unfold Mem.alloc in HA. rewrite A in HA. inv HA.
+             cbn. rewrite PMap.gso; eauto.
+          -- rewrite H6.
+             unfold Mem.alloc in HB. rewrite H1 in HB.
+             inv HB. cbn. rewrite PMap.gso; eauto.
+      + apply Mem.nextblock_alloc in HA.
+        apply Mem.nextblock_alloc in HB.
+        rewrite HA. rewrite HB. rewrite HNB.
+        symmetry. apply Pos.max_r.
+        etransitivity; eauto. rewrite HNB. lia.
+      + apply alloc_flag_join_l; eauto.
+        * apply Mem.alloc_flag_alloc2 in HA. easy.
+        * apply Mem.alloc_flag_alloc2 in HB. easy.
+        * apply Mem.nextblock_alloc in HA. rewrite HA.
+          etransitivity; eauto. rewrite HNB. lia.
+  Qed.
+
+  Opaque Mem.alloc.
+
+  Lemma bind_parameters_join:
+    Monotonic
+      (@bind_parameters)
+      (- ==> - ==> join m ++> - ==> - ==> set_le (join m)).
+  Proof.
+    repeat rstep. intros ? ?. revert y H.
+    induction H0.
+    - eexists. split. econstructor. eauto.
+    - intros. exploit assign_loc_join; eauto.
+      intros (? & ? & ?).
+      exploit IHbind_parameters. eauto.
+      intros (? & ? & ?).
+      eexists. split; eauto. econstructor; eauto.
+  Qed.
+
+  Lemma alloc_variables_join:
+    Monotonic
+      (@alloc_variables)
+      (- ==> - ==> join m ++> - ==> - ==> set_le (join m)).
+  Proof.
+    repeat rstep. intros ? ?. revert y H.
+    induction H0.
+    - intros. eexists. split. econstructor. eauto.
+    - intros. transport H. destruct x0. destruct H3. cbn in *. subst.
+      exploit IHalloc_variables. eauto.
+      intros (? & ? & ?).
+      eexists. split; eauto. econstructor; eauto.
+  Qed.
+
+End JOIN_PROP.
