cklr/RTLrel.v
@@ -235,8 +235,8 @@ Proof.
   - inv H8.
     transport_hyps; eexists; split; [ eapply c; eauto; fail | ].
     exists w'; split; rauto.
-  - edestruct cklr_alloc as (w' & Hw' & Halloc); eauto.
-    transport e. clear Halloc. transport FIND.
+  - transport e. destruct x. destruct H0. cbn in *.
+    transport FIND.
     eexists; split. eapply c; eauto; fail.
     exists w'; split. rauto.
     repeat rstep.
@@ -272,14 +272,15 @@ Global Instance semantics_rel R:
   Monotonic (@RTL.semantics) (- ==> forward_simulation (cc_c R) (cc_c R)).
 Proof.
   intros p. constructor. econstructor; auto.
+  { intros i; intuition auto. }
   intros se1 se2 w Hse1 Hse. cbn -[semantics] in *.
   eapply forward_simulation_step with (match_states := klr_diam tt (state_rel R) w).
-  - cbn. intros q1 q2 Hq. eapply (Genv.is_internal_match (ctx := p)).
-    + eapply (match_prog p).
-    + eapply match_stbls_proj; eauto.
-    + cbn. congruence.
-    + destruct Hq. cbn. auto.
-    + destruct Hq. cbn. auto.
+  (* - cbn. intros q1 q2 Hq. eapply (Genv.is_internal_match (ctx := p)). *)
+  (*   + eapply (match_prog p). *)
+  (*   + eapply match_stbls_proj; eauto. *)
+  (*   + cbn. congruence. *)
+  (*   + destruct Hq. cbn. auto. *)
+  (*   + destruct Hq. cbn. auto. *)
   - intros q1 q2 s1 Hq. destruct 1. inv Hq. cbn.
     eassert (Hge: genv_match p R w _ _) by (red; rauto).
     transport H.
