driver/CallConv.v
@@ -366,6 +366,9 @@ Program Definition lessdef_c : callconv li_c li_c :=
     match_query _ := lessdef_c_mq;
     match_reply _ := lessdef_c_mr;
   |}.
+Next Obligation. reflexivity. Qed.
+Next Obligation. inv H0. intuition auto. Qed.
+Next Obligation. inv H. intuition auto. Qed.
 
 Lemma lessdef_c_cklr R:
   cceqv (lessdef_c @ cc_c R) (cc_c R).
@@ -425,6 +428,9 @@ Program Definition lessdef_loc :=
     match_query := lessdef_loc_mq;
     match_reply := lessdef_loc_mr;
   |}.
+Next Obligation. reflexivity. Qed.
+Next Obligation. inv H0. intuition auto. Qed.
+Next Obligation. inv H. intuition auto. Qed.
 
 Lemma lessdef_loc_cklr R:
   cceqv (lessdef_loc @ cc_locset R) (cc_locset R).
@@ -617,6 +623,10 @@ Program Definition cc_locset_mach: callconv li_locset li_mach :=
     match_query := cc_locset_mach_mq;
     match_reply := cc_locset_mach_mr;
   |}.
+Next Obligation. reflexivity. Qed.
+Next Obligation. inv H0. intuition auto. Qed.
+Next Obligation. inv H. intuition auto. Qed.
+
 
 (** ** Commutation property *)
 
@@ -760,6 +770,8 @@ Instance ext_mixable:
 Proof.
   intros sz sp1 sp2 [ ] m1 m2 [ ] m1'_ m2'_ m2' _ Hsp Hm Hm'_ UPD UNCH EXT OOR _ VB.
   uncklr.
+  assert (Hflag: Mem.alloc_flag m1 = Mem.alloc_flag m1'_).
+  { destruct Hm, Hm'_, UNCH, UPD. congruence. }
   destruct (classic (sz > 0 /\ exists sb1 sofs1, sp1 = Vptr sb1 sofs1)).
   - destruct H as (SZ & sb1 & sofs1 & Hsp1). subst. inv Hsp.
     assert (Mem.mixable m1'_ sb1 m1). {
@@ -778,7 +790,7 @@ Proof.
       * eapply Mem.extends_extends_compose; eauto.
       * eapply Mem.unchanged_on_implies; eauto.
         intros _ ofs [-> Hofs] VLD. constructor; eauto.
-    + eapply Mem.unchanged_on_implies; eauto using Mem.mix_updated.
+    + eapply Mem.unchanged_on_implies. eapply Mem.mix_updated; eauto.
       inversion 1; auto.
     + eapply Mem.unchanged_on_implies; eauto using Mem.mix_unchanged.
       intros _ ofs NIA _ [<- Hofs]. apply NIA. constructor; auto.
@@ -796,6 +808,7 @@ Proof.
         unfold offset_sarg in *. xomega.
       * destruct 1; eelim H; eauto. split; eauto.
         unfold offset_sarg in *. xomega.
+      * apply Hflag.
     + apply Mem.unchanged_on_refl.
     + reflexivity.
 Qed.
@@ -804,6 +817,8 @@ Instance inj_mixable:
   Mixable inj.
 Proof.
   intros sz sp1 sp2 w m1 m2 w' m1'_ m2'_ m2' Hw Hsp Hm Hm'_ UPD UNCH EXT OOR SZ VB.
+  assert (Hflag: Mem.alloc_flag m1 = Mem.alloc_flag m1'_).
+  { destruct Hm, Hm'_. destruct H, H0, UPD, UNCH. congruence. }
   destruct SZ as [k Hk]; subst.
   destruct (classic (k > 0 /\ exists sb1 sofs1, sp1 = Vptr sb1 sofs1)).
   - destruct H as (Hk & sb1 & sofs1 & Hsp1). subst. inv Hsp.
@@ -857,6 +872,7 @@ Proof.
         unfold offset_sarg in H3. xomega.
       * destruct 1; eelim H; eauto. split; eauto.
         unfold offset_sarg in H3. xomega.
+      * apply Hflag.
     + apply Mem.unchanged_on_refl.
     + reflexivity.
 Qed.
@@ -940,6 +956,7 @@ Proof.
   - intros. destruct (classic (Mem.perm m b ofs Max Nonempty)); auto. left.
     erewrite Mem.unchanged_on_perm; eauto.
     eapply Mem.perm_valid_block; eauto.
+  - destruct UNCH. congruence.
 Qed.
 
 (** With this, we can state and prove the commutation property. *)
@@ -1319,5 +1336,3 @@ Proof.
   subst. inv Hq. inv Hq1. inv Hq2. inv Hr. inv Hr2. constructor.
   intros. eapply val_has_type_inject; eauto. red. eauto.
 Qed.
-
-
